simplify var representation

cava/Cava/Arrow/ExprEquiv.v
@@ -7,25 +7,24 @@ Set Implicit Arguments.
 Set Asymmetric Patterns.
 
   Section Equivalence.
-    Inductive obj_tup : Type := obj_pair : Kind -> Kind -> obj_tup.
-    Variables var1 var2 : Kind -> Kind -> Type.
+    Variables var1 var2 : Kind -> Type.
 
-    Definition vars := existT (fun '(obj_pair x y) => (var1 x y * var2 x y)%type).
-    Definition ctxt := list { '(obj_pair x y) : obj_tup & (var1 x y * var2 x y)%type }.
+    Definition vars := existT (fun t => (var1 t * var2 t)%type).
+    Definition ctxt := list { t : Kind & (var1 t * var2 t)%type }.
 
     Inductive kappa_equivalence:
       forall i o, ctxt
       -> kappa var1 i o -> kappa var2 i o
       -> Prop :=
-    | Var_equiv : forall i o (n1: var1 i o) (n2: var2 i o) E,
-      In (vars (obj_pair i o) (pair n1 n2)) E
+    | Var_equiv : forall x (n1: var1 x) (n2: var2 x) E,
+      In (vars (pair n1 n2)) E
       -> kappa_equivalence E (Var n1) (Var n2)
 
     | Abs_equiv : forall x y z
-      (f1: var1 Unit x -> kappa var1 y z)
-      (f2: var2 Unit x -> kappa var2 y z)
+      (f1: var1 x -> kappa var1 y z)
+      (f2: var2 x -> kappa var2 y z)
       (E: ctxt),
-      (forall n1 n2, kappa_equivalence (vars (obj_pair Unit x) (pair n1 n2) :: E) (f1 n1) (f2 n2))
+      (forall n1 n2, kappa_equivalence (vars (pair n1 n2) :: E) (f1 n1) (f2 n2))
       -> kappa_equivalence E (Abs f1) (Abs f2)
 
     | App_equiv : forall E x y z
@@ -46,14 +45,14 @@ Set Asymmetric Patterns.
     | Prim_equiv : forall E p, kappa_equivalence E (ExprSyntax.Primitive p) (ExprSyntax.Primitive p)
 
     | Letrec_equiv : forall x y z
-      (v1: var1 Unit x -> kappa var1 Unit x)
-      (v2: var2 Unit x -> kappa var2 Unit x)
-      (f1: var1 Unit x -> kappa var1 y z)
-      (f2: var2 Unit x -> kappa var2 y z)
+      (v1: var1 x -> kappa var1 Unit x)
+      (v2: var2 x -> kappa var2 Unit x)
+      (f1: var1 x -> kappa var1 y z)
+      (f2: var2 x -> kappa var2 y z)
       (E: ctxt),
-      (forall n1 n2, kappa_equivalence (vars (obj_pair Unit x) (pair n1 n2) :: E) (v1 n1) (v2 n2))
+      (forall n1 n2, kappa_equivalence (vars (pair n1 n2) :: E) (v1 n1) (v2 n2))
       ->
-      (forall n1 n2, kappa_equivalence (vars (obj_pair Unit x) (pair n1 n2) :: E) (f1 n1) (f2 n2))
+      (forall n1 n2, kappa_equivalence (vars (pair n1 n2) :: E) (f1 n1) (f2 n2))
       ->
       kappa_equivalence E (LetRec v1 f1) (LetRec v2 f2)
 
